---
title: "HW2-task1&2a"
date: "1/28/2022"
output: html_document
---

```{r setup, include=FALSE}
knitr::opts_chunk$set(echo = TRUE)
```

## Task 1
# Part a
$$
\begin{aligned} 


Z \sim N(\omega, \tau^2)  \text{ where} \ Z \in[-\gamma,\gamma]  \\

\mathbb{E}[Z\mathbb{1}_{\begin{equation} \mid Z \mid \leq \gamma\end{equation}}] &= \int^\gamma_{-\gamma} z f(z)  d z \\

&= \int^\gamma_{-\gamma} (z -\omega) \frac{1}{\sqrt{2\pi}\tau} e^{-\frac{(z-\omega)^2}{2\tau^2}} dz +\omega\int^\gamma_{-\gamma}\frac{1}{\sqrt{2\pi}\tau}e^{-\frac{(z-\omega)^2}{2\tau^2}}dz \\

&=\frac{\tau}{\sqrt{2\pi}}(e^{-\frac{(\gamma+\omega)^2}{2\tau^2}}-e^{-\frac{(\gamma-\omega)^2}{2\tau^2}})+\omega[\Phi(\frac{\gamma-\omega}{\tau})-\Phi(\frac{-\gamma-\omega}{\tau})]\\

\text{QED}

\end{aligned}

$$



# Part b

$$
\begin{aligned}
\mathbb{E}[(X-\hat\mu^{H}_{n})] &= \mathbb{E}[(X-\overline{X}_n\mathbb{1}_{ \mid \overline{X}_n \mid \geq \alpha})^2] \\
&=\mathbb{E}[(X-\overline{X}_n+\overline{X}_n-\overline{X}_n \mathbb{1}_{\mid \overline{X}_n\mid\geq\alpha})^2] \\
&= \mathbb{E}[(X-\overline{X}_n)^2]+2\mathbb{E}[(X-\overline{X}_n)(\overline{X}_n-\overline{X}_n\mathbb{1}_{\mid \overline{X}_n\mid \geq\alpha})]+\mathbb{E}[(\overline{X}_n-\overline{X}_n\mathbb{1}_{\mid \overline{X}_n\mid \geq\alpha})^2] \\

\text{Where } \mathbb{E}[\overline{X}_n]=\mathbb{E}[X] &= \mu \\ \mathbb{E}[X^2] &= \sigma^2 +\mu \\ Var(\overline{X}_n) &=
\frac{\sigma^2}{n} \\ \mathbb{E}[\overline{X}_n^2] &= \mu^2 +\frac{\sigma^2}{n} \\
\text{Thus, } \\
\mathbb{E}[(X-\overline{X}_n)^2] &= \mathbb{E}[X^2-2X\overline{X}_n+\overline{X}_n^2] \\
&=\sigma^2+\mu-2\mu^2+\mu^2+\frac{\sigma^2}{n} \\ 
&=\sigma^2+\frac{\sigma^2}{n} \\


\text{Appling the fact }\mathbb{E}(Z\mathbb{1}_{\mid Z \mid\geq\gamma}) = \mathbb{E}(Z)-\mathbb{E}(Z\mathbb{1}_{\mid Z\mid\leq\gamma})\text{ in our equation.}\\
\\

2\mathbb{E}[(X-\overline{X}_n)(\overline{X}_n-\overline{X}_n\mathbb{1}_{\mid \overline{X}_n\mid \geq\alpha})] &= 2\mathbb{E}[X(\overline{X}_n-\overline{X}_n\mathbb{1}_{\mid \overline{X}_n \mid\geq\alpha})-\overline{X}_n(\overline{X}_n-\overline{X}_n\mathbb{1}_{\mid \overline{X}_n \mid\geq\alpha})]\\

&= 2[\mu\mathbb{E}(\overline{X}_n-\overline{X}_n\mathbb{1}_{\mid \overline{X}_n\mid\geq\alpha})-\mathbb{E}(\overline{X}_n^2)+\mathbb{E}(\overline{X}_n^2\mathbb{1}_{\mid \overline{X}_n\mid\geq\alpha})] \\

\text{Appling the equation mentioned above }\Rightarrow &=2[\mu\mathbb{E}(\overline{X}_n\mathbb{1}_{\mid \overline{X}_n\mid\leq\alpha})-\frac{\sigma^2}{n}-\mu^2+\mathbb{E}(\overline{X}_n^2\mathbb{1}_{\mid \overline{X}_n\mid\geq\alpha})] \\
\\

\text{By utilizing the result from part a, we can see that }\\

\mathbb{E}(\overline{X}_n\mathbb{1}_{\mid \overline{X}_n\mid\leq\alpha}) 
&= \frac{\sigma}{\sqrt{2\pi n}}(e^{-\frac{n(\alpha+\mu)^2}{2\sigma^2}}-e^{-\frac{n(\alpha-\mu)^2}{2\sigma^2}})
+\mu(\Phi(\frac{\sqrt{n}(\alpha-\mu)}{\sigma})-\Phi(\frac{\sqrt{n}(-\alpha-\mu)}{\sigma}))\\\\

\text{Thus, }\\

2\mathbb{E}[(X-\overline{X}_n)(\overline{X}_n-\overline{X}_n\mathbb{1}_{\mid \overline{X}_n\mid \geq\alpha})] &= 
2[\mu(\frac{\sigma}{\sqrt{2\pi n}}(e^{-\frac{n(\alpha+\mu)^2}{2\sigma^2}}-e^{-\frac{n(\alpha-\mu)^2}{2\sigma^2}})
+\mu(\Phi(\frac{\sqrt{n}(\alpha-\mu)}{\sigma})-\Phi(\frac{\sqrt{n}(-\alpha-\mu)}{\sigma})))-\frac{\sigma^2}{n}-\mu^2+\mathbb{E}(\overline{X}_n^2\mathbb{1}_{\mid \overline{X}_n\mid\geq\alpha})]\\


\mathbb{E}[(\overline{X}_n-\overline{X}_n\mathbb{1}_{\mid \overline{X}_n\mid \geq\alpha})^2] &= \mathbb{E}[\overline{X}_n^2-2\overline{X}_n^2\mathbb{1}_{\mid \overline{X}_n\mid \geq\alpha}+\overline{X}_n^2\mathbb{1}^2_{\mid \overline{X}_n\mid \geq\alpha}]\\

&= \mathbb{E}(\overline{X}_n^2) - \mathbb{E}(\overline{X}_n^2\mathbb{1}_{\mid \overline{X}_n\mid \geq\alpha}) \\
&= \mu^2+\frac{\sigma^2}{n}-\mathbb{E}(\overline{X}_n^2\mathbb{1}_{\mid \overline{X}_n\mid \geq\alpha})


\end{aligned}
$$

$$
\begin{aligned}
\text{Then we can find } \mathbb{E}(\overline{X}_n^2\mathbb{1}_{\mid \overline{X}_n\mid \geq\alpha}) \text{by using the method in part a.}\\

\text{We can find } \mathbb{E}(Z^2\mathbb{1}_{\mid Z\mid\geq\gamma}) \text{ first.}\\







\end{aligned}
$$

## Task 2
# Part a

$$

\begin{aligned}

Var(Y) &= Var(X^{\top}\beta^* + \epsilon) \\

&= Var(X^{\top}\beta^*) +Var(\epsilon) \\
&= \beta^{*^{\top}}\Sigma(\rho)\beta^*+\sigma^2 \\

P(Y-X^{\top}\beta^*) &=  P(\epsilon)^2 \\
&= \sigma^2 \\

1-\frac{\sigma^2}{\beta^{*^{\top}}\Sigma(\rho)\beta^*+\sigma^2} &= \gamma \\
1-\gamma &= \frac{\sigma^2}{\beta^{*^{\top}}\Sigma(\rho)\beta^*+\sigma^2} \\

\Rightarrow 

\sigma^2 &= \frac{\beta^{*^{\top}}\Sigma(\rho)\beta^*}{\gamma}-\beta^{*^{\top}}\Sigma(\rho)\beta^* \\
&=\frac{1-\gamma}{\gamma}\beta^{*^{\top}}\Sigma(\rho)\beta^* \\

QED

\end{aligned}



$$